src/lib/communication/DY.Lib.Communication.RequestResponse.Lemmas.fst
@@ -31,28 +31,26 @@ let get_response_label tr req_meta_data = get_label #default_crypto_usages tr re
 
 val comm_meta_data_knowable: {|crypto_invariants|} -> trace -> principal -> comm_meta_data -> prop
 let comm_meta_data_knowable #cinvs tr prin req_meta_data =
-  is_knowable_by (principal_label prin) tr req_meta_data.id /\
   is_knowable_by (principal_label prin) tr req_meta_data.key
+
 
 val compute_request_message_proof:
   {|crypto_invariants|} ->
   tr:trace ->
   client:principal -> server:principal ->
-  id:bytes -> payload:bytes -> key:bytes ->
+  payload:bytes -> key:bytes ->
   Lemma
   (requires
-    is_secret (comm_label client server) tr id /\
     is_secret (comm_label client server) tr key /\
     is_knowable_by (comm_label client server) tr payload
   )
   (ensures
-    is_knowable_by (comm_label client server) tr (compute_request_message client id payload key)
+    is_knowable_by (comm_label client server) tr (compute_request_message payload key)
   )
-let compute_request_message_proof #invs tr client server id payload key =
-  serialize_wf_lemma request_message (is_knowable_by (comm_label client server) tr) {client; id; payload; key};
+let compute_request_message_proof #invs tr client server payload key =
+  serialize_wf_lemma request_message (is_knowable_by (comm_label client server) tr) {payload; key};
   ()
 
-//#push-options "--fuel 4 --ifuel 4 --z3rlimit 50"
 val send_request_proof:
   {|protocol_invariants|} ->
   tr:trace ->
@@ -79,32 +77,23 @@ let send_request_proof #invs tr comm_keys_ids higher_layer_preds client server p
     let (key, tr') = mk_rand (AeadKey comm_layer_aead_tag empty) (comm_label client server) 32 tr in
     let (id, tr') = mk_rand NoUsage (comm_label client server) 32 tr' in
     let (sid, tr') = new_session_id client tr' in
-    let ((), tr') = set_state client sid (ClientSendRequest {id; server; payload; key} <: communication_states) tr' in
+    let ((), tr') = set_state client sid (ClientSendRequest {server; payload; key} <: communication_states) tr' in
     higher_layer_preds.send_request_later tr tr' client server payload (get_label tr' key);
-    let ((), tr') = trigger_event client (CommClientSendRequest client server id payload key) tr' in
+    let ((), tr') = trigger_event client (CommClientSendRequest client server payload key) tr' in
     ()
   )
   | (Some _, tr_out) -> (
     let (key, tr') = mk_rand (AeadKey comm_layer_aead_tag empty) (comm_label client server) 32 tr in
     let (id, tr') = mk_rand NoUsage (comm_label client server) 32 tr' in
-    
     let (sid, tr') = new_session_id client tr' in
-    let ((), tr') = set_state client sid (ClientSendRequest {id; server; payload; key} <: communication_states) tr' in
-    
+    let ((), tr') = set_state client sid (ClientSendRequest {server; payload; key} <: communication_states) tr' in
     higher_layer_preds.send_request_later tr tr' client server payload (get_label tr' key);
-    assert(is_knowable_by (comm_label client server) tr' payload);
-    assert(higher_layer_preds.send_request tr' client server payload (get_label tr' key));
-    let ((), tr') = trigger_event client (CommClientSendRequest client server id payload key) tr' in
-    assert(event_triggered tr' client (CommClientSendRequest client server id payload key));
-    assert(trace_invariant tr');
-
-    compute_request_message_proof tr' client server id payload key;
-    let req_payload = compute_request_message client id payload key in
-
-    assert(request_response_event_preconditions.send_conf tr' client server req_payload);
-    send_confidential_proof #invs tr' request_response_event_preconditions comm_keys_ids client server req_payload;
-    
+    let ((), tr') = trigger_event client (CommClientSendRequest client server payload key) tr' in
+    compute_request_message_proof tr' client server payload key;
+    let req_payload = compute_request_message payload key in
+    send_confidential_proof #invs tr' request_response_event_preconditions comm_keys_ids client server req_payload;   
     let (Some msg_id, tr') = send_confidential comm_keys_ids client server req_payload tr' in
+
     assert(tr_out == tr');
     assert(trace_invariant tr_out);
     ()
@@ -122,9 +111,8 @@ val decode_request_message_proof:
   (ensures (
     match decode_request_message msg_bytes with
     | None -> True
-    | Some {id; client=client'; payload; key} -> (
+    | Some {payload; key} -> (
       exists client.
-        is_knowable_by (comm_label client server) tr id /\
         is_knowable_by (comm_label client server) tr payload /\
         is_knowable_by (comm_label client server) tr key
     )
@@ -132,10 +120,9 @@ val decode_request_message_proof:
 let decode_request_message_proof #cinvs tr server msg_bytes =
   match decode_request_message msg_bytes with
   | None -> ()
-  | Some {id; client=client'; payload; key} -> (
+  | Some {payload; key} -> (
     eliminate exists client. is_knowable_by (comm_label client server) tr msg_bytes
     returns (exists client.
-        is_knowable_by (comm_label client server) tr id /\
         is_knowable_by (comm_label client server) tr payload /\
         is_knowable_by (comm_label client server) tr key)
     with _. (
@@ -144,8 +131,7 @@ let decode_request_message_proof #cinvs tr server msg_bytes =
     )
   )
 
-
-#push-options "--fuel 0 --ifuel 0 --z3rlimit 20"
+#push-options "--z3rlimit 20"
 val receive_request_proof:
   {|protocol_invariants|} ->
   tr:trace ->
@@ -166,10 +152,7 @@ val receive_request_proof:
     | (None, tr_out) -> trace_invariant tr_out
     | (Some (payload, req_meta_data), tr_out) -> (
       trace_invariant tr_out /\
-      (*exists client. 
-        is_knowable_by (comm_label client server) tr_out payload) /\*)
-      event_triggered tr_out server (CommServerReceiveRequest server req_meta_data.id payload req_meta_data.key) /\
-      //state_was_set tr_out server sid (ServerReceiveRequest {id; client; payload; key} <: communication_states)     
+      event_triggered tr_out server (CommServerReceiveRequest server payload req_meta_data.key) /\    
       is_comm_response_payload tr_out server req_meta_data payload
     )
   ))
@@ -181,83 +164,17 @@ let receive_request_proof #invs tr comm_keys_ids higher_layer_preds server msg_i
     let (Some req_msg_bytes, tr') = receive_confidential comm_keys_ids server msg_id tr in
     decode_request_message_proof tr' server req_msg_bytes;
     let Some req_msg = decode_request_message req_msg_bytes in    
-    FStar.Classical.move_requires (parse_wf_lemma request_message (is_publishable tr')) req_msg_bytes;        
-    (*assert(trace_invariant tr');
-    assert(exists client.
-      request_response_event_preconditions.send_conf tr' client server req_msg_bytes \/
-      is_publishable tr' req_msg_bytes
-    );
-
-    assert(exists client.
-      event_triggered tr' client (CommClientSendRequest client server id payload req_msg.key) \/
-        is_publishable tr' req_msg.key
-    );
-    assert(is_knowable_by (get_label tr req_msg.key) tr' req_msg.id);*)
-
-    let ((), tr') = trigger_event server (CommServerReceiveRequest server req_msg.id req_msg.payload req_msg.key) tr' in
-    assert(event_triggered tr' server (CommServerReceiveRequest server req_msg.id req_msg.payload req_msg.key));
-
+    FStar.Classical.move_requires (parse_wf_lemma request_message (is_publishable tr')) req_msg_bytes;
+    let ((), tr') = trigger_event server (CommServerReceiveRequest server req_msg.payload req_msg.key) tr' in
     let (sid', tr') = new_session_id server tr' in
-    let ((), tr') = set_state server sid' (ServerReceiveRequest {id=req_msg.id; payload=req_msg.payload; key=req_msg.key} <: communication_states) tr' in
+    let ((), tr') = set_state server sid' (ServerReceiveRequest {payload=req_msg.payload; key=req_msg.key} <: communication_states) tr' in
     
     assert(tr' == tr_out);
-    assert(trace_invariant tr_out);
-    assert(is_comm_response_payload tr_out server req_meta_data payload);    
+    assert(trace_invariant tr_out);   
     ()
   )
 #pop-options
 
-
-val compute_response_message_proof:
-  {|crypto_invariants|} ->
-  tr:trace ->
-  client:principal -> server:principal ->
-  key:bytes -> nonce:bytes -> id:bytes -> payload:bytes ->
-  Lemma
-  (requires
-    has_communication_layer_reqres_crypto_predicates /\
-    is_knowable_by (principal_label server) tr key /\
-    is_knowable_by (get_label tr key) tr id /\
-    is_knowable_by (get_label tr key) tr payload /\    
-    is_publishable tr nonce /\
-    (key `has_usage tr` (AeadKey comm_layer_aead_tag empty) \/
-      is_publishable tr key    
-    ) /\
-    event_triggered tr server (CommServerSendResponse server id payload)
-  )
-  (ensures
-    is_publishable tr (compute_response_message client server key nonce id payload)
-  )
-let compute_response_message_proof #cinvs tr client server key nonce id payload =
-  let res:response_message = {id; payload} in
-  let res_bytes = serialize response_message res in
-  serialize_wf_lemma response_message (is_knowable_by (get_label tr key) tr) res;
-  assert(bytes_invariant tr res_bytes);
-  let ad:authenticated_data = {client; server} in
-  let ad_bytes = serialize authenticated_data ad in
-  serialize_wf_lemma authenticated_data (is_publishable tr) ad;
-  let ciphertext = aead_enc key nonce res_bytes ad_bytes in  
-  // Needed for the case that the key is publishable
-  FStar.Classical.move_requires (aead_enc_preserves_publishability tr key nonce res_bytes) ad_bytes;
-  assert(bytes_invariant tr ciphertext);
-  serialize_wf_lemma response_envelope (is_publishable tr) {nonce; ciphertext};
-  ()
-
-// TODO should this go into the core?
-(*
-val state_was_set_grows:
-  #a:Type -> {|ev:local_state a|} ->
-  tr1:trace -> tr2:trace ->
-  prin:principal -> sid:state_id -> e:a  ->
-  Lemma
-  (requires state_was_set tr1 prin sid e /\ tr1 <$ tr2)
-  (ensures state_was_set tr2 prin sid e)
-  [SMTPat (state_was_set tr1 prin sid e); SMTPat (tr1 <$ tr2)]
-let state_was_set_grows #a #ev tr1 tr2 prin sid e =
-  reveal_opaque (`%state_was_set) (state_was_set #a);
-  reveal_opaque (`%DY.Lib.State.Tagged.tagged_state_was_set) (DY.Lib.State.Tagged.tagged_state_was_set);
-  ()
-*)
 
 val mk_comm_layer_response_nonce_proof:
   {|protocol_invariants|} ->
@@ -279,6 +196,39 @@ val mk_comm_layer_response_nonce_proof:
   ))
 let mk_comm_layer_response_nonce_proof #invs tr server req_meta_data usg = ()
 
+
+val compute_response_message_proof:
+  {|crypto_invariants|} ->
+  tr:trace ->
+  server:principal ->
+  key:bytes -> nonce:bytes -> payload:bytes ->
+  Lemma
+  (requires
+    has_communication_layer_reqres_crypto_predicates /\
+    is_knowable_by (principal_label server) tr key /\
+    is_knowable_by (get_label tr key) tr payload /\    
+    is_publishable tr nonce /\
+    (key `has_usage tr` (AeadKey comm_layer_aead_tag empty) \/
+      is_publishable tr key    
+    ) /\
+    event_triggered tr server (CommServerSendResponse server payload)
+  )
+  (ensures
+    is_publishable tr (compute_response_message server key nonce payload)
+  )
+let compute_response_message_proof #cinvs tr server key nonce payload =
+  let res:response_message = {payload} in
+  let res_bytes = serialize response_message res in
+  serialize_wf_lemma response_message (is_knowable_by (get_label tr key) tr) res;
+  let ad:authenticated_data = {server} in
+  let ad_bytes = serialize authenticated_data ad in
+  serialize_wf_lemma authenticated_data (is_publishable tr) ad;
+  let ciphertext = aead_enc key nonce res_bytes ad_bytes in  
+  // Needed for the case that the key is publishable
+  FStar.Classical.move_requires (aead_enc_preserves_publishability tr key nonce res_bytes) ad_bytes;
+  serialize_wf_lemma response_envelope (is_publishable tr) {nonce; ciphertext};
+  ()
+
 val send_response_proof:
   {|protocol_invariants|} ->
   tr:trace ->
@@ -293,13 +243,6 @@ val send_response_proof:
     higher_layer_preds.send_response tr server payload /\
     has_communication_layer_state_predicates /\
     is_comm_response_payload tr server req_meta_data payload
-    (*
-      match get_state server sid tr with
-      | (Some (ServerReceiveRequest {id; client; payload=payload'; key}), tr_out) -> (
-        is_knowable_by (get_label tr key) tr payload
-      )
-      | _ -> False
-    *)
   )
   (ensures (
     let (_, tr_out) = send_response comm_keys_ids server req_meta_data payload tr in
@@ -310,34 +253,11 @@ let send_response_proof #invs tr comm_keys_ids higher_layer_preds server req_met
   | (None, tr_out) -> ()
   | (Some msg_id, tr_out) -> (
     let (Some state, tr') = get_state server req_meta_data.sid tr in
-    let ServerReceiveRequest srr = state in
-    assert(srr.key = req_meta_data.key);
-    assert(srr.id = req_meta_data.id);
-
-    assert(
-      req_meta_data.key `has_usage tr'` (AeadKey comm_layer_aead_tag empty) \/
-        is_publishable tr' req_meta_data.key
-    );
-
-    assert(is_comm_response_payload tr' server req_meta_data payload);
-    assert(get_label tr payload `can_flow tr'` get_label #default_crypto_usages tr req_meta_data.key);
-    assert(bytes_invariant tr' payload);
-    assert(is_knowable_by (get_label #default_crypto_usages tr' req_meta_data.key) tr' payload);
-    
-    let ((), tr') = trigger_event server (CommServerSendResponse server req_meta_data.id payload) tr' in
-    assert(trace_invariant tr');
-
-    
+    let ServerReceiveRequest srr = state in    
+    let ((), tr') = trigger_event server (CommServerSendResponse server payload) tr' in    
     let (nonce, tr') = mk_rand NoUsage public 32 tr' in
-
-    assert(
-      is_knowable_by (principal_label server) tr' req_meta_data.key /\
-      is_knowable_by (get_label tr req_meta_data.key) tr' req_meta_data.id /\
-      is_knowable_by (get_label tr req_meta_data.key) tr' payload
-    );
-
-    compute_response_message_proof tr' req_meta_data.client server req_meta_data.key nonce req_meta_data.id payload;
-    let resp_msg_bytes = compute_response_message req_meta_data.client server req_meta_data.key nonce req_meta_data.id payload in
+    compute_response_message_proof tr' server req_meta_data.key nonce payload;
+    let resp_msg_bytes = compute_response_message server req_meta_data.key nonce payload in
     let (msg_id, tr') = send_msg resp_msg_bytes tr' in
     assert(tr_out == tr');
     assert(trace_invariant tr_out);
@@ -350,7 +270,7 @@ val decode_response_proof:
   {|crypto_invariants|} ->
   tr:trace ->
   client:principal -> server:principal ->
-  key:bytes -> id:bytes -> msg_bytes:bytes ->
+  key:bytes -> msg_bytes:bytes ->
   Lemma
   (requires
     has_communication_layer_reqres_crypto_predicates /\
@@ -359,28 +279,23 @@ val decode_response_proof:
     key `has_usage tr` (AeadKey comm_layer_aead_tag empty)
   )
   (ensures (
-    match decode_response_message client server key id msg_bytes with
+    match decode_response_message server key msg_bytes with
     | None -> True
     | Some payload -> (
       is_knowable_by (get_label tr key) tr payload /\
-      (event_triggered tr server (CommServerSendResponse server id payload)
+      (event_triggered tr server (CommServerSendResponse server payload)
         \/ is_corrupt tr (principal_label client) \/ is_corrupt tr (principal_label server))
     )
   ))
-let decode_response_proof #cinvs tr client server key id msg_bytes =
-  match decode_response_message client server key id msg_bytes with
+let decode_response_proof #cinvs tr client server key msg_bytes =
+  match decode_response_message server key msg_bytes with
   | None -> ()
   | Some payload -> (
     parse_wf_lemma response_envelope (is_publishable tr) msg_bytes;
     let Some {nonce; ciphertext} = parse response_envelope msg_bytes in
-    assert(is_publishable tr nonce);
-    assert(is_publishable tr ciphertext);
-    serialize_wf_lemma authenticated_data (is_publishable tr) {client; server};
-    let ad_bytes = serialize authenticated_data {client; server} in
-    assert(is_publishable tr ad_bytes);
+    serialize_wf_lemma authenticated_data (is_publishable tr) {server};
+    let ad_bytes = serialize authenticated_data {server} in
     let Some res_bytes = aead_dec key nonce ciphertext ad_bytes in
-    assert(bytes_invariant tr res_bytes);
-    assert(is_knowable_by (comm_label client server) tr res_bytes);
     parse_wf_lemma response_message (is_knowable_by (comm_label client server) tr) res_bytes;
     ()
   )
@@ -406,7 +321,7 @@ val receive_response_proof:
     | (None, tr_out) -> trace_invariant tr_out
     | (Some (payload, _), tr_out) -> (
       trace_invariant tr_out /\
-      event_triggered tr_out client (CommClientReceiveResponse client req_meta_data.server req_meta_data.id payload req_meta_data.key)
+      event_triggered tr_out client (CommClientReceiveResponse client req_meta_data.server payload req_meta_data.key)
     )
   ))
 let receive_response_proof #invs tr comm_keys_ids higher_layer_preds client req_meta_data msg_id =
@@ -414,19 +329,14 @@ let receive_response_proof #invs tr comm_keys_ids higher_layer_preds client req_
   | (None, tr_out) -> ()
   | (Some (payload, _), tr_out) -> (
     let server = req_meta_data.server in
-    let id = req_meta_data.id in
     let key = req_meta_data.key in
     let (Some state, tr') = get_state client req_meta_data.sid tr in
     let ClientSendRequest csr = state in
     let (Some resp_msg_bytes, tr') = recv_msg msg_id tr' in
-    decode_response_proof tr' client csr.server csr.key csr.id resp_msg_bytes;
-    let Some payload = decode_response_message client csr.server csr.key csr.id resp_msg_bytes in
-
-    let ((), tr') = set_state client req_meta_data.sid (ClientReceiveResponse {id=csr.id; server=csr.server; payload; key=csr.key} <: communication_states) tr' in
-    assert(trace_invariant tr');
-    let ((), tr') = trigger_event client (CommClientReceiveResponse client csr.server csr.id payload csr.key) tr' in
-    assert(trace_invariant tr');
-    assert(event_triggered tr' client (CommClientReceiveResponse client csr.server csr.id payload csr.key));
+    decode_response_proof tr' client csr.server csr.key resp_msg_bytes;
+    let Some payload = decode_response_message csr.server csr.key resp_msg_bytes in
+    let ((), tr') = set_state client req_meta_data.sid (ClientReceiveResponse {server=csr.server; payload; key=csr.key} <: communication_states) tr' in
+    let ((), tr') = trigger_event client (CommClientReceiveResponse client csr.server payload csr.key) tr' in
 
     assert(tr_out == tr');
     assert(trace_invariant tr_out);
